wip prettifying swap_locals

bedrock2/src/bedrock2Examples/LiveVerif/swap.v
@@ -1,4 +1,5 @@
 Require Import bedrock2Examples.LiveVerif.string_to_ident.
+Require Import bedrock2Examples.LiveVerif.ident_to_string.
 
 Load LiveVerif.
 
@@ -37,6 +38,12 @@ Load LiveVerif.
       wp_cmd call cmd.skip t m l post.
   Proof. intros. constructor. assumption. Qed.
 
+  (* to avoid using `remember` and having to control which occurrence we want to remember *)
+  Lemma wp_locals_put: forall call c x v t m l post,
+      (forall a, a = v -> wp_cmd call c t m (map.put l x a) post) ->
+      wp_cmd call c t m (map.put l x v) post.
+  Proof. auto. Qed.
+
   Definition vc_func call '(innames, outnames, body) (t: trace) (m: mem) (argvs: list word)
                      (post : trace -> mem -> list word -> Prop) :=
     exists l, map.of_list_zip innames argvs = Some l /\
@@ -44,18 +51,40 @@ Load LiveVerif.
         exists retvs, map.getmany_of_list l' outnames = Some retvs /\ post t' m' retvs).
 
 Ltac make_fresh x :=
-  (* TODO: if there's a hypothesis called eg value_of_x, also rename it into value_of_x0 *)
   tryif is_var x then let x' := fresh x "0" in rename x into x' else idtac.
 
 Definition current_locals_marker(l: locals): locals := l.
+Definition arguments_marker(args: list word): list word := args.
+
+Declare Scope live_scope.
+Delimit Scope live_scope with live.
+
+Inductive ignore_above_this_line := mk_ignore_above_this_line.
+Notation "'ignore' 'above' 'this' 'line' : '____'" := ignore_above_this_line
+  (only printing) : live_scope.
+
+(* intro-and-position *)
+Ltac intro_p n :=
+  lazymatch goal with
+  | separator: ignore_above_this_line |- forall _: @word.rep _ _, _ =>
+    intro n; move n after separator (* after-wrt-moving-direction = above *)
+  | |- forall _: _, _ => intro n
+  end.
+
+Ltac intro_p_autonamed :=
+  lazymatch goal with
+  | |- forall x: ?T, _ => let n := fresh x in intro_p n
+  end.
+
+Ltac intros_p := repeat intro_p_autonamed.
 
 Ltac put_into_current_locals :=
   lazymatch goal with
   | |- wp_cmd _ _ _ _ (map.put ?l ?x ?v) _ =>
     let i := string_to_ident x in
     make_fresh i;
-    let n := fresh "value_of_" i in
-    remember v as i eqn: n in |- *
+    let n := fresh "L0" in
+    apply wp_locals_put; intro_p i; intro_p n
   end;
   lazymatch goal with
   | cl := current_locals_marker (reconstruct _ _) |- _ =>
@@ -68,21 +97,44 @@ Ltac put_into_current_locals :=
       let values := eval vm_compute in (tuple.of_list values) in
       change (let cl := current_locals_marker (reconstruct keys values) in
               wp_cmd call c t m cl post);
-      intro
+      intro cl;
+      lazymatch goal with
+      | arguments := arguments_marker _ |- _ =>
+        move cl before arguments (* before-wrt-moving-direction = below *)
+      end
     end
   end.
 
+Ltac map_with_ltac f l :=
+  lazymatch l with
+  | ?h :: ?t =>
+    let t' := map_with_ltac f t in
+    let h' := f h in constr:(h' :: t')
+  | nil => open_constr:(@nil _)
+  end.
+
 Ltac start :=
+  let eargnames := open_constr:(_: list string) in
+  refine (existT _ (eargnames, _, _) _);
   let call := fresh "call" in
   intro call;
-  let n := fresh "____TODO_hide_defs_above____" in
-  pose proof tt as n;
-  intros;
+  let n := fresh "____" in pose proof mk_ignore_above_this_line as n;
+  intros_p;
   (* since the arguments will get renamed, it is useful to have a list of their
      names, so that we can always see their current renamed names *)
   lazymatch goal with
   | |- vc_func ?call ?f ?t ?m ?argvalues ?post =>
-    let arguments := fresh "arguments" in pose argvalues as arguments
+    let arguments := fresh "arguments" in pose (arguments_marker argvalues) as arguments;
+    let argnames := map_with_ltac varconstr_to_string argvalues in
+    unify eargnames argnames
+  end;
+  unfold vc_func;
+  lazymatch goal with
+  | |- exists l, map.of_list_zip ?keys ?values = Some l /\ _ =>
+    let values := eval vm_compute in (tuple.of_list values) in
+    let cl := fresh "current_locals" in
+    refine (let cl := current_locals_marker (reconstruct keys values) in ex_intro _ cl _);
+    split; [reflexivity|]
   end.
 
 Ltac assign name val :=
@@ -90,8 +142,14 @@ Ltac assign name val :=
   eapply wp_var; [ reflexivity |];
   put_into_current_locals.
 
-Declare Scope live_scope.
-Delimit Scope live_scope with live.
+Ltac ret retnames :=
+  eapply wp_skip;
+  lazymatch goal with
+  | |- exists _, map.getmany_of_list _ ?eretnames = Some _ /\ _ =>
+    unify eretnames retnames;
+    eexists; split; [reflexivity|]
+  end.
+
 Open Scope live_scope.
 
 Notation "'ready' 'for' 'next' 'command'" := (wp_cmd _ _ _ _ _ _)
@@ -108,42 +166,54 @@ Notation "[ x ; y ; .. ; z ]" :=
 
 Notation "l" := (current_locals_marker (reconstruct _ l%reconstruct_locals))
   (at level 100, only printing) : live_scope.
+Notation "l" := (arguments_marker l)
+  (at level 100, only printing) : live_scope.
 
 (* end move *)
 
 
 (* TODO: write down postcondition only at end *)
-Definition swap: {f: list string * list string * cmd &
+Definition swap_locals: {f: list string * list string * cmd &
   forall call t m a b,
     vc_func call f t m [a; b] (fun t' m' retvs =>
       t' = t /\ m' = m /\ retvs = [b; a]
   )}.
   (* note: we could just return ["b", "a"] and then the body would be just skip *)
-  refine (existT _ (["a"; "b"], ["res1"; "res2"], _) _).
   start.
-  unfold vc_func. letexists. split. {
-    subst l.
-    transitivity (Some (current_locals_marker (reconstruct ["a"; "b"]
-                   (PrimitivePair.pair.mk a (PrimitivePair.pair.mk b tt))))).
-    all: reflexivity.
-  }
-  rename l into current_locals, m into current_mem.
+
+  rename m into current_mem, t into current_trace.
+  move current_trace after ____.
+  move current_mem after ____.
 
   assign "t" "a".
   assign "a" "b".
   assign "b" "t".
   assign "res1" "a".
   assign "res2" "b".
-
-  eapply wp_skip.
-  eexists. ssplit; reflexivity.
+  ret ["res1"; "res2"].
+  subst. auto.
 Defined.
 
+(* TODO: write down postcondition only at end *)
+Definition swap: {f: list string * list string * cmd &
+  forall call t m a_addr b_addr a b R,
+    (scalar a_addr a * scalar b_addr b * R)%sep m ->
+    vc_func call f t m [a_addr; b_addr] (fun t' m' retvs =>
+      t' = t /\ (scalar a_addr b * scalar b_addr a * R)%sep m' /\ retvs = []
+  )}.
+  start.
+
+  Undelimit Scope live_scope.
+  Close Scope live_scope.
+
+  (* Scalars.store_word_of_sep *)
+Abort.
+
 Goal False.
-  let r := eval unfold swap in match swap with
-                               | existT _ f _ => f
-                               end
-    in pose r.
+  let r := eval unfold swap_locals in
+  match swap_locals with
+  | existT _ f _ => f
+  end in pose r.
 Abort.
 
 Definition foo(a b: word): word := a ^+ b.
