bedrock2/src/bedrock2Examples/LiveVerif/ident_to_string.v
@@ -1,0 +1,84 @@
+Require Import Coq.Strings.String.
+Require Import Ltac2.Ltac2.
+Require Ltac2.Option.
+
+(* Takes a list of powers instead of one power and dividing because
+   Ltac2 does not have integer division: https://github.com/coq/coq/issues/13802 *)
+Ltac2 rec int_to_bits_rec(powers: int list)(val: int) :=
+  match powers with
+  | p :: rest =>
+    if Int.le p val
+    then true :: int_to_bits_rec rest (Int.sub val p)
+    else false :: int_to_bits_rec rest val
+  | [] => []
+  end.
+
+(* [2^(n-1); ..., 2^0] *)
+Ltac2 rec powers_of_two(n: int) :=
+  if Int.equal n 1 then [1] else
+  let r := powers_of_two (Int.sub n 1) in
+  match r with
+  | h :: t => Int.mul 2 h :: r
+  | [] => []
+  end.
+
+Ltac2 char_to_bits(c: char) :=
+  int_to_bits_rec (powers_of_two 8) (Char.to_int c).
+
+Ltac2 bool_to_coq(b: bool) :=
+  if b then constr:(true) else constr:(false).
+
+Ltac2 mkApp(f: constr)(args: constr array) :=
+  Constr.Unsafe.make (Constr.Unsafe.App f args).
+
+Ltac2 char_to_ascii(c: char) :=
+  mkApp constr:(Ascii.Ascii)
+        (Array.of_list (List.rev (List.map bool_to_coq (char_to_bits c)))).
+
+Ltac2 rec string_to_coq_rec(s: string)(i: int)(acc: constr) :=
+  if Int.lt i 0 then acc else
+    let c := char_to_ascii (String.get s i) in
+    string_to_coq_rec s (Int.sub i 1) constr:(String.String $c $acc).
+
+Ltac2 string_to_coq(s: string) :=
+  string_to_coq_rec s (Int.sub (String.length s) 1) constr:(String.EmptyString).
+
+Ltac2 ident_to_coq(i: ident) := string_to_coq (Ident.to_string i).
+
+Ltac2 varconstr_to_coq(c: constr) :=
+  match Constr.Unsafe.kind c with
+  | Constr.Unsafe.Var i => ident_to_coq i
+  | _ => Control.throw_invalid_argument "not a Constr.Unsafe.Var"
+  end.
+
+(* Test:
+   Ltac2 Eval string_to_coq "hello world".
+   Goal forall a: nat, a = a. intros.
+   Ltac2 Eval varconstr_to_coq constr:(a).
+*)
+
+Inductive PassStringFromLtac2ToLtac1 := mkPassStringFromLtac2ToLtac1 (s: string).
+
+Ltac2 pose_varconstr_as_wrapped_string(c: constr) :=
+  let s := varconstr_to_coq c in pose (mkPassStringFromLtac2ToLtac1 $s).
+
+Ltac pose_varconstr_as_wrapped_string :=
+  ltac2:(s |- pose_varconstr_as_wrapped_string (Option.get (Ltac1.to_constr s))).
+
+Ltac varconstr_to_string c :=
+  let __ := match constr:(Set) with
+            | _ => pose_varconstr_as_wrapped_string c
+            end in
+  match goal with
+  | x := mkPassStringFromLtac2ToLtac1 ?s |- _ =>
+    let __ := match constr:(Set) with _ => clear x end in s
+  end.
+
+Local Open Scope string_scope.
+Set Default Proof Mode "Classic".
+Goal forall my_var: nat, my_var = my_var.
+  intros.
+  match goal with
+  | |- _ = ?x => let r := varconstr_to_string x in pose r
+  end.
+Abort.
